progress on finite_iff_to_singular_finite, replaced hardcoded states with constants, finished accepts_iff_singular_accepts

eNFA_Regex_equivalence_other.lean
@@ -281,18 +281,22 @@ lemma dont_go_nowhere (A : εNFA alphabet ℕ) (hAempty : A.start = ∅) : A.acc
     simp [hAempty] at h_s₁ -- contradiction
 
 
+def SingularStart  := 2
+def SingularAccept := 0
+
 def to_singular (A : εNFA alphabet ℕ) : εNFA alphabet ℕ := {
-    start  := { 2 }
-    accept := { 4 }
+    start  := { SingularStart }
+    accept := { SingularAccept }
     step   := fun q c =>
+        let A' := A.to_1mod2
         if q % 2 = 1 then
-            if q ∈ (εNFA.to_1mod2 A).accept && c = none then
-                    (εNFA.to_1mod2 A).step q c ∪ { 4 }
+            if q ∈ A'.accept && c = none then
+                A'.step q c ∪ { SingularAccept }
             else
-                (εNFA.to_1mod2 A).step q c
+                A'.step q c
         else
-            if q = 2 && c = none then
-                (εNFA.to_1mod2 A).start
+            if q = SingularStart && c = none then
+                A'.start
             else
                 ∅
     : εNFA alphabet ℕ
@@ -310,7 +314,6 @@ lemma to_singular_contains (A: εNFA alphabet ℕ): (to_singular A).contains A.t
     all_goals simp only [subset_insert, subset_refl, empty_subset]
 
 
-
 lemma accepts_iff_singular_accepts (A : εNFA alphabet ℕ) (A' : εNFA alphabet ℕ) (hA': A' = to_singular A) :
     A.accepts = A'.accepts := by
     rw [@Language.ext_iff]
@@ -321,19 +324,19 @@ lemma accepts_iff_singular_accepts (A : εNFA alphabet ℕ) (A' : εNFA alphabet
         rw[@εNFA.mem_accepts_iff_exists_path] at h_A_accepts_x ⊢
 
         obtain ⟨ s, a, x', hs, ha, hx', hApath⟩ := h_A_accepts_x
-        use 2, 4, ([none] ++ x' ++ [none])
+        use SingularStart, SingularAccept, ([none] ++ x' ++ [none])
 
         refine ⟨ by subst hA'; rfl, by subst hA'; rfl,
             by simp only [List.nil_append, List.reduceOption_cons_of_none, List.reduceOption_append, List.reduceOption_nil, List.append_nil, hx']
             , ?_ ⟩
 
-        have hfirst: A'.IsPath 2 (2*s + 1) [none] := by
+        have hfirst: A'.IsPath SingularStart (2*s + 1) [none] := by
             subst hA'
-            simp [to_singular, εNFA.to_1mod2, hs]
+            simp [to_singular, εNFA.to_1mod2, hs, SingularStart]
 
-        have hlast: A'.IsPath (2*a + 1) 4 [none] := by
+        have hlast: A'.IsPath (2*a + 1) SingularAccept [none] := by
             subst hA'
-            simp [to_singular, εNFA.to_1mod2, ha]
+            simp [to_singular, εNFA.to_1mod2, ha, SingularAccept]
 
         have hmiddle: A'.IsPath (2*s + 1) (2*a + 1) x' := by
             subst hA'
@@ -354,12 +357,12 @@ lemma accepts_iff_singular_accepts (A : εNFA alphabet ℕ) (A' : εNFA alphabet
         rw[@εNFA.mem_accepts_iff_exists_path] at h_A'_accepts_x ⊢
         obtain ⟨ s', a', x', h_s'_start, h_a'_accept, h_x', hA'path ⟩ := h_A'_accepts_x
 
-        have h_s'_2: s' = 2 := by
+        have h_s'_2: s' = SingularStart := by
             subst hA'
             simp [to_singular] at h_s'_start
             exact h_s'_start
 
-        have h_a'_4: a' = 4 := by
+        have h_a'_4: a' = SingularAccept := by
             subst hA'
             simp [to_singular] at h_a'_accept
             exact h_a'_accept
@@ -369,17 +372,12 @@ lemma accepts_iff_singular_accepts (A : εNFA alphabet ℕ) (A' : εNFA alphabet
         clear h_s'_start h_a'_accept
 
         cases hA'path
-        case cons s _ y' h_step h_path_s_4 =>
-            simp [hA', to_singular] at h_step
-            obtain ⟨ h, h_s_start ⟩ := h_step
-            subst h
+        case cons s σ y' h_step h_path_s_accept =>
+            simp [hA', to_singular, SingularStart, SingularAccept] at h_step
+            obtain ⟨ ⟨ _, h_σ_none ⟩ , h_s_start ⟩ := h_step
 
-            have first_transition_is_to_odd_state: s % 2 = 1:= by
-                have hmod: (A.to_1mod2).is_1mod2 := by
-                    exact⟨A,rfl⟩
-                exact εNFA.if_1mod2_qs_is_1mod2 A.to_1mod2 hmod s h_s_start
-
-
+            have first_transition_is_to_odd_state: s % 2 = 1:=
+                A.to_1mod2.if_1mod2_qs_is_1mod2 ⟨A, rfl⟩ s h_s_start
 
             have h_temp: ∀ (q q': ℕ) (σ : Option alphabet), (q % 2 = 1) → (q' % 2 = 1) → (q' ∈ A'.step q σ )
             → (q' ∈ A.to_1mod2.step q σ ) := by
@@ -390,6 +388,7 @@ lemma accepts_iff_singular_accepts (A : εNFA alphabet ℕ) (A' : εNFA alphabet
                 · simp [hacc] at hstep ⊢
                   rcases hstep with h | h
                   · exfalso
+                    simp[SingularAccept] at h
                     omega
                   · exact h
                 · simp [hacc] at hstep ⊢
@@ -399,48 +398,202 @@ lemma accepts_iff_singular_accepts (A : εNFA alphabet ℕ) (A' : εNFA alphabet
 
             --next step: path between odds in A' is odd
             --next step: odd path in A' -> odd path in A1
-            have odd_step_in_1mod2_stays_odd :
-              ∀ (q q' : ℕ) (σ : Option alphabet),
-                q % 2 = 1 →
-                q' ∈ (A.to_1mod2).step q σ →
-                q' % 2 = 1 := by
-              intro q q' σ hq_odd hstep
-              sorry
 
-            have path_to_four :
-              ∀ {q : ℕ} {y : List (Option alphabet)},
-                q % 2 = 1 →
-                (to_singular A).IsPath q 4 y →
-                ∃ qf mid,
-                  qf ∈ (A.to_1mod2).accept ∧
-                  (A.to_1mod2).IsPath q qf mid ∧
-                  y = mid ++ [none] := by
-                  sorry
+            have path_to_singular_accept (q : ℕ) (y : List (Option alphabet))
+                (h_q_1mod2: q % 2 = 1) (h_path : A'.IsPath q SingularAccept y) :
+                ∃ qf mid, qf ∈ (A.to_1mod2).accept ∧ (A.to_1mod2).IsPath q qf mid ∧ y = mid ++ [none] := by
+                induction y generalizing q
+                case nil =>
+                    simp only [εNFA.isPath_nil] at h_path
+                    simp [SingularAccept] at h_path
+                    omega
+                case cons c tail h_induction =>
+                    cases h_path
+                    case cons t h_step h_path =>
+                        by_cases tail = []
+                        case pos h_tail_empty =>
+                            clear h_induction
+                            subst h_tail_empty
+                            simp only [εNFA.isPath_nil] at h_path
+                            subst h_path
 
-            have h_path_s_4' : (to_singular A).IsPath s 4 y' := by
-                simpa [hA'] using h_path_s_4
+                            have h_c_none : c = none := by
+                                simp [hA', to_singular, h_q_1mod2] at h_step
+                                split_ifs at h_step
+                                case pos h_none => exact h_none.right
+                                case neg =>
+                                    have : SingularAccept % 2 = 1 :=
+                                        (A.to_1mod2.if_1mod2_step_is_1mod2 ⟨A,rfl⟩ q SingularAccept c h_step).right
+                                    simp [SingularAccept] at this -- contradiction
+                            subst h_c_none
+
+                            use q, []
+                            simp only [εNFA.isPath_nil, List.nil_append, and_self, and_true]
+
+                            simp [hA', to_singular, h_q_1mod2] at h_step
+                            split_ifs at h_step
+                            case pos h_q_accept => exact h_q_accept
+                            case neg =>
+                                have : SingularAccept % 2 = 1 :=
+                                        (A.to_1mod2.if_1mod2_step_is_1mod2 ⟨A,rfl⟩ q SingularAccept none h_step).right
+                                simp [SingularAccept] at this -- contradiction
+
+                        case neg h_tail_nonempty =>
+                            have h_t_1mod2 : t % 2 = 1 := by
+                                cases h_path
+                                case nil => contradiction
+                                case cons t' c' tail' h_step' h_path' =>
+                                    have h_t_not_SAS : t ≠ SingularAccept := by
+                                        by_contra!
+                                        subst this
+
+                                        have h_step'_empty : A'.step SingularAccept c' = ∅ := by
+                                            simp [hA', to_singular, SingularAccept, SingularStart]
+
+                                        simp [h_step'_empty] at h_step' --contradiction
+
+                                    simp [hA', to_singular, h_q_1mod2] at h_step
+                                    split_ifs at h_step
+                                    case pos h_accept =>
+                                        simp [h_t_not_SAS] at h_step
+                                        exact (A.to_1mod2.if_1mod2_step_is_1mod2 ⟨A, rfl⟩ q t c h_step).right
+                                    case neg => exact (A.to_1mod2.if_1mod2_step_is_1mod2 ⟨A, rfl⟩ q t c h_step).right
+
+                            obtain ⟨ qf, mid', h_induction ⟩ := h_induction t h_t_1mod2 h_path
+                            use qf, c :: mid'
+                            simp [h_induction]
+                            replace h_induction := h_induction.right.left
+                            simp [hA', to_singular, h_q_1mod2] at h_step
+                            split_ifs at h_step
+                            case pos =>
+                                have : t ≠ SingularAccept := by simp [SingularAccept]; omega
+                                simp [this] at h_step
+                                apply A.to_1mod2.isPath_singleton.mpr at h_step
+                                exact A.to_1mod2.isPath_append.mpr ⟨ t, h_step, h_induction⟩
+                            case neg =>
+                                apply A.to_1mod2.isPath_singleton.mpr at h_step
+                                exact A.to_1mod2.isPath_append.mpr ⟨ t, h_step, h_induction⟩
 
             obtain ⟨qf, mid, h_qf_accept, h_mid_path, h_y'_eq⟩ :=
-              path_to_four (q := s) (y := y') first_transition_is_to_odd_state h_path_s_4'
+              path_to_singular_accept (q := s) (y := y') first_transition_is_to_odd_state h_path_s_accept
 
             have h_mid : mid.reduceOption = x := by
-                simp at h_x'
-                rw [h_y'_eq, List.reduceOption_append] at h_x'
-                simpa using h_x'
+                simp only [h_y'_eq, List.reduceOption_cons_of_none, List.reduceOption_append,
+                  List.reduceOption_nil, List.append_nil] at h_x'
+                exact h_x'
 
             use s, qf, mid
 
 
-def max_reachable_node_n (A : εNFA alphabet ℕ) (n : ℕ) :=
+def εNFA.max_reachable_node (A : εNFA alphabet ℕ) (n : ℕ) :=
     (∃s₁: ℕ, ∃x: List (Option alphabet), s₁ ∈ A.start ∧ A.IsPath s₁ n x)
     ∧
     ∀n': ℕ, (n' > n) → ¬(∃s₁: ℕ, ∃x: List (Option alphabet), s₁ ∈ A.start ∧ A.IsPath s₁ n' x)
 
-def is_finite_automata (A : εNFA alphabet ℕ) :=
-    (A.start = ∅) ∨ (A.start ≠ ∅ ∧ (∃n: ℕ, max_reachable_node_n A n))
+def εNFA.is_finite_automata (A : εNFA alphabet ℕ) :=
+    (A.start = ∅) ∨ (∃n: ℕ, A.max_reachable_node n)
 
 lemma finite_iff_to_singular_finite (A : εNFA alphabet ℕ) (A' : εNFA alphabet ℕ) (hA': A' = to_singular A):
-    is_finite_automata A ↔ is_finite_automata A' := by sorry
+    A.is_finite_automata ↔ A'.is_finite_automata := by
+
+    unfold εNFA.is_finite_automata
+    constructor
+    case mp =>
+        rintro (h_start_empty | h_max_reachable)
+        case inl =>
+            right
+            replace h_start_empty : A.to_1mod2.start = ∅ := by
+                simp [εNFA.to_1mod2, h_start_empty]
+
+            use SingularStart
+            unfold εNFA.max_reachable_node
+            constructor
+            case h.left =>
+                use SingularStart, []
+                simp [hA', to_singular]
+            case h.right =>
+                intro n' h_n'
+                by_contra!
+                obtain ⟨ s₁, x, h ⟩ := this
+                have : s₁ = SingularStart := by
+                    replace h := h.left
+                    simp [hA', to_singular] at h
+                    exact h
+                subst this
+                replace h := h.right
+                cases h
+                case nil => contradiction
+                case cons t c x' h_step h_path =>
+                    simp [hA', to_singular, h_start_empty, SingularStart] at h_step
+
+        case inr =>
+            right
+            obtain ⟨ n, h_n ⟩ := h_max_reachable
+
+            unfold εNFA.max_reachable_node at h_n ⊢
+
+            obtain ⟨ ⟨ q, x, h_q_start, h_path_q_n_x ⟩, h_n_max ⟩ := h_n
+            let q₂ := 2*q + 1
+            let n₂ := 2*n + 1
+            rw [A.path_iff_1mod2_path A.to_1mod2 q n q₂ n₂ x] at h_path_q_n_x
+
+            have h_A'_contains_A_1mod2 := to_singular_contains A
+            rw[← hA'] at h_A'_contains_A_1mod2
+
+            by_cases n > SingularStart
+            case pos =>
+                use n₂
+                constructor
+                case left =>
+                    use SingularStart, [none] ++ x
+                    refine ⟨ by simp [hA', to_singular], ?_ ⟩
+                    have h_step: q₂ ∈ A'.step SingularStart none := by
+                        simp [hA', to_singular, SingularStart, εNFA.to_1mod2, q₂, h_q_start]
+                    apply A'.isPath_singleton.mpr at h_step
+
+                    have := A'.path_if_contains A.to_1mod2 h_A'_contains_A_1mod2 q₂ n₂ x h_path_q_n_x
+
+                    exact A'.isPath_append.mpr ⟨ q₂, h_step, this ⟩
+
+                case right =>
+                    intro n' h_n'
+
+                    --replace h_n_max := h_n_max n' (by omega)
+                    simp at h_n_max ⊢
+                    intro s' h_s' x
+
+                    simp [hA', to_singular] at h_s'
+                    subst h_s'
+
+                    by_contra!
+                    cases this
+                    case nil =>
+                        omega
+                    case cons t' c tail h_step h_path =>
+                        have h_t_start: t' ∈ A.to_1mod2.start := by
+                            simp [hA', to_singular, SingularStart] at h_step
+                            exact h_step.right
+
+                        absurd h_n_max
+                        simp
+                        simp [εNFA.to_1mod2] at h_t_start
+                        obtain ⟨ t, h_t'_start, h_t ⟩ := h_t_start
+
+                        sorry
+            case neg =>
+                use SingularStart
+                constructor
+                case left =>
+                    use SingularStart, []
+                    simp [hA', to_singular]
+                case right =>
+                    intro n' h_n'
+                    by_contra!
+                    absurd h_n_max
+                    -- todo...
+                    sorry
+    case mpr =>
+        sorry
 
 def to_trim (A : εNFA alphabet ℕ) (i j k : ℕ) : εNFA alphabet ℕ := {
     start  := { i }
@@ -460,8 +613,8 @@ def is_trim (A' : εNFA alphabet ℕ) (i' j' k' : ℕ) :=
     ∃ (A : εNFA alphabet ℕ), A' = to_trim A i' j' k'
 
 lemma singular_finite_accepts_iff_trim_accepts (A A': εNFA alphabet ℕ) (s a n: ℕ)
-(hAsingular: is_singular A) (hAfinite: is_finite_automata A)
-(hn_max: max_reachable_node_n A n) (hs_start: is_alone_in_set A.start s) (ha_accept: is_alone_in_set A.accept a)
+(hAsingular: is_singular A) (hAfinite: A.is_finite_automata)
+(hn_max: A.max_reachable_node n) (hs_start: is_alone_in_set A.start s) (ha_accept: is_alone_in_set A.accept a)
 (hA'istrim: A' = to_trim A s a n):
     A.accepts = A'.accepts := by sorry
 
@@ -480,12 +633,12 @@ def regex_for_path_from_i_to_j_through_k (A : εNFA alphabet ℕ) (i j k : ℕ) 
         else
             character_list_to_regex characters
     else
-        let r₁ := regex_for_path_from_i_to_j_through_k A i j (k-1)
-        let r₂ := regex_for_path_from_i_to_j_through_k A i k (k-1)
-        let r₃ := regex_for_path_from_i_to_j_through_k A k k (k-1)
-        let r₄ := regex_for_path_from_i_to_j_through_k A k j (k-1)
+        let rᵢⱼ := regex_for_path_from_i_to_j_through_k A i j (k-1)
+        let rᵢₖ := regex_for_path_from_i_to_j_through_k A i k (k-1)
+        let rₖₖ := regex_for_path_from_i_to_j_through_k A k k (k-1)
+        let rₖⱼ := regex_for_path_from_i_to_j_through_k A k j (k-1)
 
-        r₁ + (r₂ * r₃.star * r₄)
+        rᵢⱼ + (rᵢₖ * rₖₖ.star * rₖⱼ)
 
 termination_by k
 decreasing_by
@@ -495,7 +648,7 @@ lemma regex_is_path (A : εNFA alphabet ℕ) (i j k : ℕ) (r: RegularExpression
     ∀(x : List alphabet), ((x ∈ r.matches') ↔ (∃(x': List ((Option alphabet))), (x'.reduceOption = x) ∧ ((to_trim A i j k).IsPath i j x'))) := by
     sorry
 
-theorem εNFA_to_Regex (A: εNFA alphabet ℕ) : is_finite_automata A → (∃ (r: RegularExpression alphabet), r.matches' = A.accepts) := by
+theorem εNFA_to_Regex (A: εNFA alphabet ℕ) : A.is_finite_automata → (∃ (r: RegularExpression alphabet), r.matches' = A.accepts) := by
     let A' := to_singular A
     have hA'tosinA: A' = to_singular A := by
         simp_all only [A']
@@ -504,33 +657,31 @@ theorem εNFA_to_Regex (A: εNFA alphabet ℕ) : is_finite_automata A → (∃ (
     simp_all only [A']
     rw [finite_iff_to_singular_finite A A' hA'tosinA]
 
-    rw [is_finite_automata]
-    rintro ( hnill | ⟨ hAStartNotEmpty, n, hnmax ⟩ )
+    rw [εNFA.is_finite_automata]
+    rintro ( hnill | ⟨ n, hnmax ⟩ )
     case inl =>
         use 0
         simp only [dont_go_nowhere A' hnill, RegularExpression.matches']
     case inr =>
         have hA'singular: is_singular A' := by
-            simp_all only [ne_eq, A']
+            simp_all only [A']
             unfold to_singular
             unfold is_singular
             constructor
-            use 2 --todo: fix if to_singular changes
+            use SingularStart
             exact ((fun a ↦ a) ∘ fun a ↦ a) rfl
-            use 4 --todo: fix if to_singular changes
+            use SingularAccept
             exact ((fun a ↦ a) ∘ fun a ↦ a) rfl
         unfold is_singular at hA'singular
         obtain ⟨ s, hs ⟩ := hA'singular.left
         obtain ⟨ a, ha ⟩ := hA'singular.right
         let A'' := to_trim A' s a n
         have histrim: A'' = to_trim A' s a n := by
-            simp_all only [ne_eq, A', A'']
-        have hA'finite: is_finite_automata A' := by
-            rw [is_finite_automata]
+            simp_all only [A', A'']
+        have hA'finite: A'.is_finite_automata := by
+            rw [εNFA.is_finite_automata]
             right
-            constructor
-            · exact hAStartNotEmpty
-            · use n
+            use n
         rw [singular_finite_accepts_iff_trim_accepts
         A' A'' s a n
         hA'singular hA'finite
@@ -539,20 +690,20 @@ theorem εNFA_to_Regex (A: εNFA alphabet ℕ) : is_finite_automata A → (∃ (
         let r' := regex_for_path_from_i_to_j_through_k A'' s a n
         have hr: r' = regex_for_path_from_i_to_j_through_k A' s a n := by
             subst A'
-            simp_all only [ne_eq, A'', r']
+            simp_all only [A'', r']
             obtain ⟨left, right⟩ := hA'singular
             obtain ⟨w, h⟩ := left
             obtain ⟨w_1, h_1⟩ := right
             --rfl
             sorry
         have hgs: A''.start = {s} := by
-            simp_all only [ne_eq, A', A'', r']
+            simp_all only [A', A'', r']
             obtain ⟨left, right⟩ := hA'singular
             obtain ⟨w, h⟩ := left
             obtain ⟨w_1, h_1⟩ := right
             rfl
         have hga: A''.accept = {a} := by
-            simp_all only [ne_eq, A', A'', r']
+            simp_all only [A', A'', r']
             obtain ⟨left, right⟩ := hA'singular
             obtain ⟨w, h⟩ := left
             obtain ⟨w_1, h_1⟩ := right
@@ -584,4 +735,4 @@ theorem εNFA_to_Regex (A: εNFA alphabet ℕ) : is_finite_automata A → (∃ (
             constructor
             · exact htempx
             subst htempx
-            simp_all only [ne_eq, mem_singleton_iff, A', A'']
+            simp_all only [mem_singleton_iff, A', A'']
